theories/Symbolic/Instantiation.v
@@ -117,7 +117,7 @@ Module Type InstantiationOn
     | term_get_slice_int t       => bv.of_Z (inst (Inst := inst_term) t ι)
     | term_unsigned t            => bv.unsigned (inst (Inst := inst_term) t ι)
     | term_truncate m t          => bv.truncate m (inst (Inst := inst_term) t ι)
-    | term_vector_subrange t s l => bv.vector_subrange (inst (Inst := inst_term) t ι) s l
+    | term_vector_subrange s l t => bv.vector_subrange s l (inst (Inst := inst_term) t ι)
     | term_negate  t             => bv.negate (inst (Inst := inst_term) t ι)
     | @term_tuple _ σs ts        =>
         envrec.of_env (inst (Inst := inst_env (InstSA := @inst_term)) ts ι)
@@ -432,7 +432,7 @@ Module Type InstantiationOn
     #[export,program] Instance proper_term_get_slice_int {Σ n} : Proper ((≡) ==> (≡)) (@term_get_slice_int Σ n).
     #[export,program] Instance proper_term_unsigned {Σ n} : Proper ((≡) ==> (≡)) (@term_unsigned Σ n).
     #[export,program] Instance proper_term_truncate {Σ n m p} : Proper ((≡) ==> (≡)) (@term_truncate Σ n m p).
-    #[export,program] Instance proper_term_vector_subrange {Σ n s l p} : Proper ((≡) ==> (≡)) (fun t => @term_vector_subrange Σ n t s l p).
+    #[export,program] Instance proper_term_vector_subrange {Σ n s l p} : Proper ((≡) ==> (≡)) (@term_vector_subrange Σ n s l p).
     #[export,program] Instance proper_term_negate {Σ n} : Proper ((≡) ==> (≡)) (@term_negate Σ n).
     #[export,program] Instance proper_term_tuple {Σ σs} : Proper ((≡) ==> (≡)) (@term_tuple Σ σs).
     #[export,program] Instance proper_term_union {Σ U K} : Proper ((≡) ==> (≡)) (@term_union Σ U K).
