theories/Symbolic/OccursCheck.v
@@ -89,7 +89,7 @@ Module Type OccursCheckOn
       | term_get_slice_int t => term_get_slice_int <$> occurs_check_term xIn t
       | term_unsigned t => term_unsigned <$> occurs_check_term xIn t
       | term_truncate m t => (fun t' => term_truncate m t') <$> occurs_check_term xIn t
-      | term_vector_subrange t s l => (fun t' => term_vector_subrange t' s l) <$> occurs_check_term xIn t
+      | term_vector_subrange s l t => term_vector_subrange s l <$> occurs_check_term xIn t
       | term_negate t => term_negate <$> occurs_check_term xIn t
       | @term_tuple _ σs ts =>
         @term_tuple _ σs <$> occurs_check (OccursCheck := occurs_check_env (OCT := @occurs_check_term)) xIn ts
